added support of external function

compiler_test/bad_programs/volatile2.c
@@ -1,0 +1,17 @@
+#include <stdio.h>
+
+volatile int shared_var = 10;  // Volatile global variable
+
+void read_from_volatile() {
+    volatile int *ptr = &shared_var;  // Pointer to volatile int
+
+    int value = *ptr;  // Dereference on RHS, ensures fresh read from memory
+
+    printf("Read value: %d\n", value);
+}
+
+int main() {
+    read_from_volatile();
+    return 0;
+}
+
